WIP: commutative monoid canonicalization wrt arbitrary congruence relation

ulib/FStar.Tactics.CanonCommMonoidSimple.Equiv.fst
@@ -87,39 +87,42 @@ let rec flatten_correct_aux (#a:Type) (eq:equiv a) (m:cm a eq) (am:amap a) (xs1 
   : Lemma (xsdenote eq m am (xs1 @ xs2) `EQ?.eq eq` CM?.mult m (xsdenote eq m am xs1)
                                                                (xsdenote eq m am xs2)) = 
   match xs1 with
-  | [] -> CM?.identity m (xsdenote eq m am xs2);
-          EQ?.symmetry eq (CM?.mult m (CM?.unit m) (xsdenote eq m am xs2)) (xsdenote eq m am xs2)
-  | [x] -> (if (Nil? xs2) 
-            then (right_identity eq m (select x am);
-                  EQ?.symmetry eq (CM?.mult m (select x am) (CM?.unit m)) (select x am))
-            else EQ?.reflexivity eq (CM?.mult m (xsdenote eq m am [x]) (xsdenote eq m am xs2)))
-  
-  | x::xs1' -> flatten_correct_aux eq m am xs1' xs2;
-               EQ?.reflexivity eq (select x am);
-               CM?.congruence m (select x am) (xsdenote eq m am (xs1' @ xs2)) 
-                                (select x am) (CM?.mult m (xsdenote eq m am xs1') (xsdenote eq m am xs2));
-               CM?.associativity m (select x am) (xsdenote eq m am xs1') (xsdenote eq m am xs2);
-               EQ?.symmetry eq (CM?.mult m (CM?.mult m (select x am) (xsdenote eq m am xs1')) (xsdenote eq m am xs2)) 
-                               (CM?.mult m (select x am) (CM?.mult m (xsdenote eq m am xs1') (xsdenote eq m am xs2)));
-               EQ?.transitivity eq (CM?.mult m (select x am) (xsdenote eq m am (xs1' @ xs2)))
-                                   (CM?.mult m (select x am) (CM?.mult m (xsdenote eq m am xs1') (xsdenote eq m am xs2)))
-                                   (CM?.mult m (CM?.mult m (select x am) (xsdenote eq m am xs1')) (xsdenote eq m am xs2))
+  | [] -> 
+      CM?.identity m (xsdenote eq m am xs2);
+      EQ?.symmetry eq (CM?.mult m (CM?.unit m) (xsdenote eq m am xs2)) (xsdenote eq m am xs2)
+  | [x] -> (
+      if (Nil? xs2) 
+      then (right_identity eq m (select x am);
+            EQ?.symmetry eq (CM?.mult m (select x am) (CM?.unit m)) (select x am))
+      else EQ?.reflexivity eq (CM?.mult m (xsdenote eq m am [x]) (xsdenote eq m am xs2)))
+  | x::xs1' -> 
+      flatten_correct_aux eq m am xs1' xs2;
+      EQ?.reflexivity eq (select x am);
+      CM?.congruence m (select x am) (xsdenote eq m am (xs1' @ xs2)) 
+                       (select x am) (CM?.mult m (xsdenote eq m am xs1') (xsdenote eq m am xs2));
+      CM?.associativity m (select x am) (xsdenote eq m am xs1') (xsdenote eq m am xs2);
+      EQ?.symmetry eq (CM?.mult m (CM?.mult m (select x am) (xsdenote eq m am xs1')) (xsdenote eq m am xs2)) 
+                      (CM?.mult m (select x am) (CM?.mult m (xsdenote eq m am xs1') (xsdenote eq m am xs2)));
+      EQ?.transitivity eq (CM?.mult m (select x am) (xsdenote eq m am (xs1' @ xs2)))
+                          (CM?.mult m (select x am) (CM?.mult m (xsdenote eq m am xs1') (xsdenote eq m am xs2)))
+                          (CM?.mult m (CM?.mult m (select x am) (xsdenote eq m am xs1')) (xsdenote eq m am xs2))
 
 let rec flatten_correct (#a:Type) (eq:equiv a) (m:cm a eq) (am:amap a) (e:exp) 
   : Lemma (mdenote eq m am e `EQ?.eq eq` xsdenote eq m am (flatten e)) = 
   match e with
   | Unit -> EQ?.reflexivity eq (CM?.unit m)
   | Atom x -> EQ?.reflexivity eq (select x am)
-  | Mult e1 e2 -> flatten_correct_aux eq m am (flatten e1) (flatten e2);
-                  EQ?.symmetry eq (xsdenote eq m am (flatten e1 @ flatten e2)) 
-                                  (CM?.mult m (xsdenote eq m am (flatten e1)) (xsdenote eq m am (flatten e2)));
-                  flatten_correct eq m am e1; 
-                  flatten_correct eq m am e2;
-                  CM?.congruence m (mdenote eq m am e1) (mdenote eq m am e2) 
-                                   (xsdenote eq m am (flatten e1)) (xsdenote eq m am (flatten e2));
-                  EQ?.transitivity eq (CM?.mult m (mdenote eq m am e1) (mdenote eq m am e2)) 
-                                      (CM?.mult m (xsdenote eq m am (flatten e1)) (xsdenote eq m am (flatten e2)))
-                                      (xsdenote eq m am (flatten e1 @ flatten e2))  
+  | Mult e1 e2 -> 
+      flatten_correct_aux eq m am (flatten e1) (flatten e2);
+      EQ?.symmetry eq (xsdenote eq m am (flatten e1 @ flatten e2)) 
+                      (CM?.mult m (xsdenote eq m am (flatten e1)) (xsdenote eq m am (flatten e2)));
+      flatten_correct eq m am e1; 
+      flatten_correct eq m am e2;
+      CM?.congruence m (mdenote eq m am e1) (mdenote eq m am e2) 
+                       (xsdenote eq m am (flatten e1)) (xsdenote eq m am (flatten e2));
+      EQ?.transitivity eq (CM?.mult m (mdenote eq m am e1) (mdenote eq m am e2)) 
+                          (CM?.mult m (xsdenote eq m am (flatten e1)) (xsdenote eq m am (flatten e2)))
+                          (xsdenote eq m am (flatten e1 @ flatten e2))  
 
 (***** Permuting the lists of atoms
        by swapping adjacent elements *)
@@ -139,20 +142,21 @@ let permute_correct (p:permute) =
 
 let swap (n:nat) :Type = x:nat{x < n-1}
 
-let rec apply_swap_aux (#a:Type) (n:nat) (xs:list a) (s:swap (length xs + n)) :
-    Pure (list a) (requires True)
+let rec apply_swap_aux (#a:Type) (n:nat) (xs:list a) (s:swap (length xs + n))
+  : Pure (list a) (requires True)
                   (ensures (fun zs -> length zs == length xs)) (decreases xs) =
   match xs with
   | [] | [_] -> xs
-  | x1 :: x2 :: xs' -> if n = (s <: nat)
-                       then x2 :: x1 :: xs'
-                       else x1 :: apply_swap_aux (n+1) (x2 :: xs') s
+  | x1 :: x2 :: xs' -> 
+      if n = (s <: nat)
+      then x2 :: x1 :: xs'
+      else x1 :: apply_swap_aux (n+1) (x2 :: xs') s
 
 let apply_swap (#a:Type) = apply_swap_aux #a 0
 
 let rec apply_swap_aux_correct (#a:Type) (n:nat) (eq:equiv a) (m:cm a eq) (am:amap a)
-                           (xs:list atom) (s:swap (length xs + n)) :
-    Lemma (requires True)
+                           (xs:list atom) (s:swap (length xs + n))
+  : Lemma (requires True)
       (ensures (xsdenote eq m am xs `EQ?.eq eq` xsdenote eq m am (apply_swap_aux n xs s)))
       (decreases xs) =
   match xs with
@@ -185,40 +189,44 @@ let rec apply_swap_aux_correct (#a:Type) (n:nat) (eq:equiv a) (m:cm a eq) (am:am
         CM?.congruence m (select x1 am) (xsdenote eq m am (x2 :: xs'))
                          (select x1 am) (xsdenote eq m am (apply_swap_aux (n+1) (x2 :: xs') s)))
 
-let apply_swap_correct (#a:Type) (m:cm a) (am:amap a)
-                       (xs:list atom) (s:swap (length xs)):
-    Lemma (ensures (xsdenote m am xs == xsdenote m am (apply_swap xs s)))
-          (decreases xs) = apply_swap_aux_correct 0 m am xs s
+let apply_swap_correct (#a:Type) (eq:equiv a) (m:cm a eq) (am:amap a)
+                       (xs:list atom) (s:swap (length xs))
+  : Lemma (ensures (xsdenote eq m am xs `EQ?.eq eq` xsdenote eq m am (apply_swap xs s)))
+          (decreases xs) = apply_swap_aux_correct 0 eq m am xs s
 
-let rec apply_swaps (#a:Type) (xs:list a) (ss:list (swap (length xs))) :
-    Pure (list a) (requires True)
+let rec apply_swaps (#a:Type) (xs:list a) (ss:list (swap (length xs))) 
+  : Pure (list a) (requires True)
                   (ensures (fun zs -> length zs == length xs)) (decreases ss) =
   match ss with
   | [] -> xs
   | s::ss' -> apply_swaps (apply_swap xs s) ss'
 
-let rec apply_swaps_correct (#a:Type) (m:cm a) (am:amap a)
-                            (xs:list atom) (ss:list (swap (length xs))):
-    Lemma (requires True)
-      (ensures (xsdenote m am xs == xsdenote m am (apply_swaps xs ss)))
+let rec apply_swaps_correct (#a:Type) (eq:equiv a) (m:cm a eq) (am:amap a)
+                            (xs:list atom) (ss:list (swap (length xs)))
+  : Lemma (requires True)
+      (ensures (xsdenote eq m am xs `EQ?.eq eq` xsdenote eq m am (apply_swaps xs ss)))
       (decreases ss) =
   match ss with
-  | [] -> ()
-  | s::ss' -> apply_swap_correct m am xs s;
-              apply_swaps_correct m am (apply_swap xs s) ss'
+  | [] -> EQ?.reflexivity eq (xsdenote eq m am xs)
+  | s::ss' -> 
+      apply_swap_correct eq m am xs s;
+      apply_swaps_correct eq m am (apply_swap xs s) ss';
+      EQ?.transitivity eq (xsdenote eq m am xs)
+                          (xsdenote eq m am (apply_swap xs s))
+                          (xsdenote eq m am (apply_swaps (apply_swap xs s) ss'))
 
 let permute_via_swaps (p:permute) =
   (#a:Type) -> (am:amap a) -> xs:list atom ->
-    Lemma (exists ss. p xs == apply_swaps xs ss)
+    Lemma (exists (ss:swaps_for xs). p xs == apply_swaps xs ss)
 
 let rec permute_via_swaps_correct_aux (p:permute) (pvs:permute_via_swaps p)
-                               (#a:Type) (m:cm a) (am:amap a) (xs:list atom) :
-    Lemma (xsdenote m am xs == xsdenote m am (p xs)) =
+                               (#a:Type) (eq:equiv a)(m:cm a eq) (am:amap a) (xs:list atom) 
+  : Lemma (xsdenote eq m am xs `EQ?.eq eq` xsdenote eq m am (p xs)) =
   pvs am xs;
-  assert(exists ss. p xs == apply_swaps xs ss);
-  exists_elim (xsdenote m am xs == xsdenote m am (p xs))
-    (() <: squash (exists ss. p xs == apply_swaps xs ss))
-    (fun ss -> apply_swaps_correct m am xs ss)
+  assert(exists (ss:swaps_for xs). p xs == apply_swaps xs ss);
+  exists_elim (xsdenote eq m am xs `EQ?.eq eq` xsdenote eq m am (p xs))
+    (() <: squash (exists (ss:swaps_for xs). p xs == apply_swaps xs ss))
+    (fun ss -> apply_swaps_correct eq m am xs ss)
 
 let permute_via_swaps_correct
   (p:permute) (pvs:permute_via_swaps p) : permute_correct p =
@@ -231,18 +239,19 @@ let permute_via_swaps_correct
 
 let sort : permute = List.Tot.sortWith #nat (compare_of_bool (<))
 
-let sort_via_swaps (#a:Type) (am : amap a)  (xs:list atom) :
-  Lemma (exists ss. sort xs == apply_swaps xs ss) =
+let sort_via_swaps (#a:Type) (am:amap a)  (xs:list atom) 
+  : Lemma (exists (ss:swaps_for xs). sort xs == apply_swaps xs ss) =
   List.Tot.Properties.sortWith_permutation #nat (compare_of_bool (<)) xs;
-  let ss = equal_counts_implies_swaps #nat xs (sort xs) in
-  assert (sort xs == apply_swaps xs ss)
-      by (dump "here"; admit1 ())
-  // this should just work from the type of ss,
+  let (ss:swaps_for xs) = equal_counts_implies_swaps #nat xs (sort xs) in
+  assume (sort xs == apply_swaps xs ss)
+  // this should just work from the type of ss 
+  // (and the postcondition of equal_counts_implies_swaps),
   // but ss gets substituted by its definition in the WP
+  // (the same already in FStar.Tactics.CanonCommMonoidSimple.fst)
 
-let rec sort_correct_aux (#a:Type) (m:cm a) (am:amap a) (xs:list atom) :
-    Lemma (xsdenote m am xs == xsdenote m am (sort xs)) =
-  permute_via_swaps_correct sort (fun #a am -> sort_via_swaps am) m am xs
+let rec sort_correct_aux (#a:Type) (eq:equiv a) (m:cm a eq) (am:amap a) (xs:list atom) 
+  : Lemma (xsdenote eq m am xs `EQ?.eq eq` xsdenote eq m am (sort xs)) =
+  permute_via_swaps_correct sort (fun #a am -> sort_via_swaps am) eq m am xs
 
 let sort_correct : permute_correct sort = (fun #a -> sort_correct_aux #a)
 
@@ -251,19 +260,31 @@ let sort_correct : permute_correct sort = (fun #a -> sort_correct_aux #a)
 [@plugin]
 let canon (e:exp) = sort (flatten e)
 
-let canon_correct (#a:Type) (m:cm a) (am:amap a) (e:exp) :
-    Lemma (mdenote m am e == xsdenote m am (canon e)) =
-  flatten_correct m am e; sort_correct m am (flatten e)
+let canon_correct (#a:Type) (eq:equiv a) (m:cm a eq) (am:amap a) (e:exp) 
+  : Lemma (mdenote eq m am e `EQ?.eq eq` xsdenote eq m am (canon e)) =
+  flatten_correct eq m am e; 
+  sort_correct eq m am (flatten e);
+  EQ?.transitivity eq (mdenote eq m am e)
+                      (xsdenote eq m am (flatten e))
+                      (xsdenote eq m am (sort (flatten e)))
 
-let monoid_reflect_orig (#a:Type) (m:cm a) (am:amap a) (e1 e2:exp) :
-  Lemma (requires (xsdenote m am (canon e1) == xsdenote m am (canon e2)))
-        (ensures (mdenote m am e1 == mdenote m am e2)) =
-  canon_correct m am e1; canon_correct m am e2
+let monoid_reflect_orig (#a:Type) (eq:equiv a) (m:cm a eq) (am:amap a) (e1 e2:exp)
+  : Lemma (requires (xsdenote eq m am (canon e1) `EQ?.eq eq` xsdenote eq m am (canon e2)))
+          (ensures (mdenote eq m am e1 `EQ?.eq eq` mdenote eq m am e2)) =
+  canon_correct eq m am e1; 
+  canon_correct eq m am e2;
+  EQ?.symmetry eq (mdenote eq m am e2) (xsdenote eq m am (canon e2));
+  EQ?.transitivity eq (mdenote eq m am e1)
+                      (xsdenote eq m am (canon e1))
+                      (xsdenote eq m am (canon e2));
+  EQ?.transitivity eq (mdenote eq m am e1)
+                      (xsdenote eq m am (canon e2))
+                      (mdenote eq m am e2)
 
-let monoid_reflect (#a:Type) (m:cm a) (am:amap a) (e1 e2:exp)
-    (_ : squash (xsdenote m am (canon e1) == xsdenote m am (canon e2)))
-       : squash (mdenote m am e1 == mdenote m am e2) =
-  canon_correct m am e1; canon_correct m am e2
+let monoid_reflect (#a:Type) (eq:equiv a) (m:cm a eq) (am:amap a) (e1 e2:exp)
+    (_ : squash (xsdenote eq m am (canon e1) `EQ?.eq eq` xsdenote eq m am (canon e2)))
+       : squash (mdenote eq m am e1 `EQ?.eq eq` mdenote eq m am e2) =
+  monoid_reflect_orig #a eq m am e1 e2
 
 (* Finds the position of first occurrence of x in xs.
    This is now specialized to terms and their funny term_eq. *)
@@ -296,52 +317,9 @@ let rec reification_aux (#a:Type) (ts:list term) (am:amap a)
     then (Unit, ts, am)
     else fatom t ts am
 
-let reification (#a:Type) (m:cm a) (ts:list term) (am:amap a) (t:term) :
+let reification (#a:Type) (eq:equiv a) (m:cm a eq) (ts:list term) (am:amap a) (t:term) :
     Tac (exp * list term * amap a) =
   let mult = norm_term [delta] (quote (CM?.mult m)) in
   let unit = norm_term [delta] (quote (CM?.unit m)) in
   let t    = norm_term [delta] t in
   reification_aux ts am mult unit t
-
-let canon_monoid (#a:Type) (m:cm a) : Tac unit =
-  norm [];
-  match term_as_formula (cur_goal ()) with
-  | Comp (Eq (Some t)) t1 t2 ->
-      // dump ("t1 =" ^ term_to_string t1 ^
-      //     "; t2 =" ^ term_to_string t2);
-      if term_eq t (quote a) then
-        let (r1, ts, am) = reification m [] (const (CM?.unit m)) t1 in
-        let (r2, _, am) = reification m ts am t2 in
-         dump ("am =" ^ term_to_string (quote am));
-        change_sq (quote (mdenote m am r1 == mdenote m am r2));
-        // dump ("before =" ^ term_to_string (norm_term [delta;primops]
-        //   (quote (mdenote m am r1 == mdenote m am r2))));
-        // dump ("expected after =" ^ term_to_string (norm_term [delta;primops]
-        //   (quote (xsdenote m am (canon r1) ==
-        //           xsdenote m am (canon r2)))));
-        apply (`monoid_reflect);
-        // dump ("after apply");
-        norm [delta_only [`%canon; `%xsdenote; `%flatten; `%sort;
-                `%select; `%assoc; `%fst; `%__proj__Mktuple2__item___1;
-                `%(@); `%append; `%List.Tot.Base.sortWith;
-                `%List.Tot.Base.partition; `%bool_of_compare; `%compare_of_bool;
-           ]; primops]
-        // ;dump "done"
-      else fail "Goal should be an equality at the right monoid type"
-  | _ -> fail "Goal should be an equality"
-
-
-
-(*
-(***** Example *)
-
-let lem0 (a b c d : int) =
-  assert_by_tactic (0 + 1 + a + b + c + d + 2 == (b + 0) + 2 + d + (c + a + 0) + 1)
-  (fun _ -> canon_monoid int_plus_cm; trefl())
-
-open FStar.Mul
-
-let _ =
-  assert_by_tactic (forall (a b c d : int). ((b + 1) * 1) * 2 * a * (c * a) * 1 == a * (b + 1) * c * a * 2)
-  (fun _ -> ignore (forall_intros()); canon_monoid int_multiply_cm; trefl())
-*)
